tools/dafny-server-docker/build-docker.sh
@@ -1,0 +1,7 @@
+#!/bin/bash
+
+#Building docker images
+#https://www.linode.com/docs/kubernetes/deploy-container-image-to-kubernetes/
+#https://training.play-with-docker.com/beginner-linux/#Task_2
+
+docker image build --tag jonhdotnet/dafny_server:1.1 dafny_server/
